WIP: defined the equivalence relations in more depth and started sketching the proof for the first two diagrams.

MicroPolicies/Merged.v
@@ -317,8 +317,9 @@ Definition encode_code_placeholder (cde : code) (pc0 : nat) : {fmap word_ordType
 Definition initial_state cde (pb : prog_buffers) (pi : Program.interface) : (Symbolic.state lrc_tags [eqType of unit]) :=
   let nc := (1+ Nat.log2 (1 + (size (domm pi)))) in
   let mem0 := (initial_memory pb) in
+  let pc0 := (size mem0) in
   let pctag := build_tpc 0 in
-  {|mem := unionm (encode_code cde (size mem0)) mem0 ; regs := reg0 ; pc := (word_of_nat 0)@pctag ; internal := tt; comp_num := nc|}.
+  {|mem := unionm (encode_code cde pc0) mem0 ; regs := reg0 ; pc := (word_of_nat pc0)@pctag ; internal := tt; comp_num := nc|}.
 
 End WithClasses.
 
