MicroPolicies/Recomposition.v
@@ -142,12 +142,15 @@ Section Recomposition.
   Definition initial_state3: state -> Prop :=
     fun s => s = initial_state (code prog'') (prog_buffers prog'') (prog_interface prog'').
   
-  Definition allowed_UB: state -> Prop :=
-    fun '(Symbolic.State m r (Types.Atom pc _) _ _) =>
+  Definition color_of: state -> option Component.id :=
+    fun '(Symbolic.State m _ (Types.Atom pc _) _ _) =>
       match (m pc) with
-      | None => False
-      | Some (Types.Atom _ tag) => (color tag) \in (domm ic)
+      | None => None
+      | Some (Types.Atom _ tag) => Some (color tag)
       end.
+    
+  Definition allowed_UB: state -> Prop :=
+    fun s => Option.apply (fun comp => (comp \in (domm ic)):Prop) False (color_of s).
 
   Definition final_state_me: state -> Prop :=
     fun '(Symbolic.State m r (Types.Atom pc _) _ _) =>
@@ -246,12 +249,7 @@ Section Recomposition.
 
     Variant side := Left | Right.
 
-    Definition color_of: state -> option Component.id :=
-      fun '(Symbolic.State m _ (Types.Atom pc _) _ _) =>
-        match (m pc) with
-        | None => None
-        | Some (Types.Atom _ tag) => Some (color tag)
-        end.
+    Definition other_side s := match s with Left => Right | Right => Left end.
 
     Definition side_of (s: state): option side :=
         do! c <- color_of s;
@@ -260,32 +258,230 @@ Section Recomposition.
            else
              Some Right.
 
+    
+    Definition is_relevant_comp i c : Prop :=
+      match i with
+      | Left => c \in domm ip
+      | Right => c \in domm ic
+      end.
+
     Definition stack_value := Types.atom (Types.mword mt) value_tag.
 
+    Fixpoint find_rank' {T} (f: pred T) (l: seq T) (n: nat) : option nat :=
+      match l with
+      | [] => None
+      | e :: l => if (f e) then Some n else find_rank' f l (S n)
+      end.
+
+    Definition find_rank {T} (f: pred T) (l: seq T) : option nat := find_rank' f l 0.
+    (* Todo: write a lemma (about find_rank) usable along get_procedures and well_formed_program *)
+    
+    Definition p0 (prog: program) (comp: Component.id): option nat :=
+      do! start <- find_rank (fun '(_,tag) => color tag == comp) (code prog);
+      Some (start + size (domm (@initial_memory mt (prog_buffers prog)))).
+    
+    Definition offset1: NMap ssrint.int :=
+      mkfmapfp (fun comp => do! p_s3 <- p0 prog'' comp; 
+                         do! p_s1 <- p0 prog comp;
+                         Some (encode_int (Z.pos_sub (Pos.of_nat p_s3) (Pos.of_nat p_s1)))) (domm ip).
+    
+    Definition offset2: NMap ssrint.int := 
+      mkfmapfp (fun comp => do! p_s3 <- p0 prog'' comp; 
+                         do! p_s2 <- p0 prog comp;
+                         Some (encode_int (Z.pos_sub (Pos.of_nat p_s3) (Pos.of_nat p_s2)))) (domm ip).
+    
     Record metadata :=
-      { stack: seq (stack_value * stack_value * stack_value)%type;
-        offset1: NMap Z;
-        offset2: NMap Z;
+      { stack: seq (stack_value * stack_value * stack_value * Component.id )%type;
+        (*
+        offset1: NMap ssrint.int;
+        offset2: NMap ssrint.int;
         offset1_complete: domm offset1 = domm ip;
-        offset2_complete: domm offset2 = domm ic;
+        offset2_complete: domm offset2 = domm ic; *)
       }.
 
+    Fixpoint correct_levels (s : seq (stack_value * stack_value * stack_value * Component.id )) : Prop :=
+      match s with
+      | [] => True
+      | ((Types.Atom _ t1), (Types.Atom _ t2), (Types.Atom _ t3), c) :: s' =>
+          t1 = t2 /\ t2 = t3 /\ t1 = Ret (size s') /\ (c \in domm ip \/ c \in domm ic) /\ correct_levels s'
+      end.
+
+    Definition contains_value (s : state) (v : stack_value) : Prop :=
+      (exists w v', mem s w = Some v' /\ v = Types.Atom (Types.vala v') (vtag (Types.taga v')) ) \/
+        (exists w v', regs s w = Some v' /\ v = Types.Atom (Types.vala v') (Types.taga v') ).
+    
+    Definition get_offset i comp :=
+      match i with
+      | Left => offset1 comp
+      | Right => offset2 comp
+      end.
+
+    Definition points_to_comp_code (s : state) (v : stack_value) (comp : Component.id) : Prop :=
+      Option.apply (fun memval => color (Types.taga (memval)) = comp) False (mem s (Types.vala v)).
+    (* this might need to check that is_code is true in some conditions *)
+    
+    Definition well_formed_metadata (i : side) (m: metadata) s s' : Prop :=
+        (correct_levels (stack m) /\
+           forall v1 v2 v3 v c off,
+             In (v1, v2, v3, c) (stack m) ->
+             (match i with Left => v1 | Right => v2 end) = v ->
+             get_offset i c = Some off ->
+             points_to_comp_code s v c /\
+               points_to_comp_code s' v3 c /\
+               (is_relevant_comp i c -> contains_value s v -> contains_value s' v3) /\
+               (is_relevant_comp i c -> (Types.vala v3) = addw (Types.vala v) (as_word off))).
+    (* todo : sanity check *)
+
+    Notation data := (Types.atom (Types.mword mt) mem_tag).
+    
+    Definition data_match (i: side) (comp: Component.id) (m: metadata) (d: stack_value) (d': stack_value) : Prop :=
+      match (d, d') with
+      | (Types.Atom v1 t1, Types.Atom v2 t2) =>
+          t1 = t2 /\
+            match t1 with
+            | Invalidated => True
+            | Other => v1 = v2
+            | InternalJump => Option.apply (fun off => v1 = addw v2 (as_word off)) False (get_offset i comp)
+            | Ret _ =>
+                match i with
+                | Left  => exists sv', In (d, sv', d', comp) (stack m)
+                | Right => exists sv', In (sv', d, d', comp) (stack m)
+                end
+            end
+      end.
+    
+    Definition data_match' (i: side) (m: metadata) (d: data) (d': data) : Prop :=
+      match (d, d') with
+      | (Types.Atom v1 t1, Types.Atom v2 t2) =>
+          t1 = t2 /\
+            let comp := (color t1) in
+            (data_match i comp m (Types.Atom v1 (vtag t1)) (Types.Atom v2 (vtag t2)))
+      end.
+    
+    Definition memory_match (i: side) (m: metadata) (s: state) (s': state) : Prop :=
+      forall w d,
+        not (is_code (Types.taga d)) ->
+        is_relevant_comp i (color (Types.taga d)) ->
+        ((mem s' w) = Some d -> exists d', data_match' i m d d' /\ (mem s  w) = Some d') /\
+          ((mem s  w) = Some d -> exists d', data_match' i m d d' /\ (mem s' w) = Some d').
+
+    Definition registers_match (i: side) (m: metadata) (s: state) (s': state) : Prop :=
+      forall c w d,
+        color_of s = Some c ->
+        ((regs s' w) = Some d -> exists d', data_match i c m d d' /\ (regs s  w) = Some d') /\
+          ((regs s  w) = Some d -> exists d', data_match i c m d d' /\ (regs s' w) = Some d').
+
+    Definition same_pc (i: side) (s: state) (s': state) : Prop :=
+      oapp
+        (fun comp => oapp (fun off => (Types.vala (pc s')) = addw (Types.vala (pc s)) (as_word off))
+                    False (get_offset i comp))
+        False (color_of s).
+
+    Definition combined_codes (i: side) (m: metadata) (s: state) (s': state) : Prop :=
+      forall w v off c,
+        is_relevant_comp i c ->
+        get_offset Left c = Some off ->
+        is_code (Types.taga v) ->
+        color (Types.taga v) = c ->
+        ((mem s' (addw w (as_word off)) = Some v) <-> (mem s w = Some v)).
+    
     Variant common_equiv: metadata -> state -> state -> state -> Prop :=
+        common_equiv_def : forall m s1 s2 s3,
+            combined_codes Left  m s1 s3 ->
+            combined_codes Right m s2 s3 ->
+            common_equiv m s1 s2 s3
     .
     Variant strong_equiv (i: side): metadata -> state -> state -> Prop :=
+      strong_equiv_def : forall m s s',
+          well_formed_metadata i m s s' ->
+          same_pc i s s' ->
+          color_of s <> None ->
+          color_of s = color_of s' ->
+          side_of s' = Some i ->
+          memory_match i m s s' ->
+          registers_match i m s s' ->
+          strong_equiv i m s s'
     .
+
     Variant weak_equiv (i: side): metadata -> state -> state -> Prop :=
+      weak_equiv_def : forall m s s',
+          well_formed_metadata i m s s' ->
+          color_of s = color_of s' ->
+          side_of s' = Some (other_side i) ->
+          memory_match i m s s' ->
+          weak_equiv i m s s'
     .
 
 
   End SimulationRelations.
 
-  Theorem simulation:
-    @threeway_simulation sem sem' sem'' (sd_traces det_sem) (sd_traces det_sem') (sd_traces det_sem'').
+  Notation match_states := (match_states sem sem' sem'' (common_equiv)
+    (strong_equiv Left) (strong_equiv Right) (weak_equiv Left) (weak_equiv Right)).
+
+  
+  Lemma match_initial_states:
+  forall s1, Smallstep.initial_state sem s1 ->
+  forall s2, Smallstep.initial_state sem' s2 ->
+  exists s3 M, Smallstep.initial_state sem'' s3 /\ match_states M s1 s2 s3.
   Proof.
-    eapply threeway_simulation_diagram.
-    - admit.
-    - admit.
+    intros s1 init1 s2 init2.
+    unfold Smallstep.initial_state, sem, sem' in init1, init2. simpl in init1. unfold initial_state1, initial_state2 in *.
+    remember (initial_state (code prog'') (prog_buffers prog'') (prog_interface prog'')) as s3.
+    exists s3. exists ({|stack := []|}).
+    split; try (simpl; unfold initial_state3; done).
+    remember (prog_main p) as main. destruct main; [eapply match_states_left | eapply match_states_right]; econstructor; simpl.
+    - unfold combined_codes. intros.
+  Admitted.
+
+  Lemma step_silent_strong1:
+  forall s1 s1', Step sem s1 E0 s1' ->
+  forall s2 s3 M, strong_equiv Left M s1 s3 ->
+           weak_equiv Right M s2 s3 ->
+      common_equiv M s1 s2 s3 ->
+  exists s3' M', Plus sem'' s3 E0 s3' /\ (* Using Plus to ensure the strongly related states take a step *)
+           strong_equiv Left M' s1' s3' /\
+           weak_equiv Right M' s2 s3' /\
+              common_equiv M' s1' s2 s3'.
+  Proof.
+    intros s1 s1' step_s1 s2 s3 M strong weak common. simpl in step_s1.
+    remember E0 as t.
+    remember (@Exec.stepf _ _ _ Merged.transfer _ table s3) as s3'.
+    destruct step_s1 as [s1 ? s1' step_2 allowed | s1 ? s1' step_1 step_2]; subst t.
+    - exfalso. unfold allowed_UB in *.
+      destruct strong as [m s1 s3 wf_m pc_s1_s3 color_ineq color_eq side_eq mem_match reg_match].
+      rewrite color_eq in allowed. remember (color_of s3) as comp.
+      destruct comp; try contradiction. simpl in *. unfold side_of in side_eq. rewrite <- Heqcomp in side_eq. simpl in side_eq.
+      remember (i \in domm ip) as cond. simpl in *. unfold Component.id in *. rewrite <- Heqcond in side_eq.
+      destruct cond; try inversion side_eq. eapply Machine.Intermediate.fdisjoint_partition_notinboth.
+      + inversion Hmergeable_ifaces as [[_ fdisj] _]. exact fdisj.
+      + exact allowed.
+      + done. 
+    - destruct s3' as [[s3' ev]|].
+      + exists s3', M. admit.
+      + exfalso. unfold step2, step1, step_mp, step_me in step_1, step_2. simpl in step_1, step_2.
+        setoid_rewrite <- Exec.stepP in step_1. setoid_rewrite <- Exec.stepP in step_2.
+        destruct strong as [m s1 s3 wf_m pc_s1_s3 color_ineq color_eq side_eq mem_match reg_match].
+        unfold same_pc in *.
+        destruct (color_of s1) as [comp|]; try contradiction; simpl in pc_s1_s3.
+        remember (offset1 comp) as off.
+        destruct off as [off|]; try contradiction; simpl in pc_s1_s3.
+        destruct common as [m s1 s2 s3 code_s1 code_s2].
+        remember (mem s1 (Types.vala (pc s1))) as instr.
+        destruct instr. admit. unfold Exec.stepf in step_1. destruct s1, pc0. simpl in *. rewrite <- Heqinstr in step_1.
+        simpl in step_1. inversion step_1.
+        destruct (code_s1 (pc s1) _ off comp).
+        admit.
+  Admitted.
+      (*Set Printing All.*) 
+
+      
+  Theorem tsim_properties_match_states:
+    @tsim_properties sem sem' sem'' (sd_traces det_sem) (sd_traces det_sem') (sd_traces det_sem'')
+      (fun s1 s2 s3 => exists M, match_states M s1 s2 s3).
+  Proof.
+    eapply threeway_simulation_properties.
+    - eapply match_initial_states.
+    - eapply step_silent_strong1.
     - admit.
     - admit.
     - admit.
@@ -302,18 +498,20 @@ Section Recomposition.
     setoid_rewrite (does_prefix_equiv det_sem').
     setoid_rewrite (does_prefix_equiv det_sem'').
     intros m dp_sem dp_sem'.
-    destruct simulation.
+    pose proof tsim_properties_match_states as props.
     inversion dp_sem; subst; inversion dp_sem'; subst;
       try (match goal with | H : (forall s : Smallstep.state _, ~ Smallstep.initial_state _ s) |- _ =>
                                exfalso; eapply H; simpl; unfold initial_state2; unfold initial_state1; eauto end);
-      try (remember (initial_state (code prog'') (prog_buffers prog'') (prog_interface prog'')) as s3;
-           (assert (match_s3: match_states s s0 s3) by 
-             ( match goal with | H : (Smallstep.initial_state sem _), H' : (Smallstep.initial_state sem' _) |- _ =>
-               destruct props as [a]; destruct (a _ _ H H') as [s3' [init match_init]]; simpl in init; unfold initial_state3 in init;
-               rewrite <- init in Heqs3; subst; done end) );
-           (match goal with | H : (Star sem' _ _ _) |- _ =>
-           destruct (tsimulation_star props H0 H s3 match_s3) as [s3' [star_sem'' ?]] end);
-           assert (init: Smallstep.initial_state sem'' s3) by done).
+      remember (initial_state (code prog'') (prog_buffers prog'') (prog_interface prog'')) as s3;
+      try (assert (match_s3: exists M, match_states M s s0 s3) by 
+          (( match goal with | H : (Smallstep.initial_state sem _), H' : (Smallstep.initial_state sem' _) |- _ =>
+                                 rename H into init_sem; rename H' into init_sem' end);
+           destruct props as [a]; destruct (a _ _ init_sem init_sem') as [s3' [init match_init]];
+           simpl in init; unfold initial_state3 in init;
+           rewrite <- init in Heqs3; subst; try done));
+      try ((match goal with | H : (Star sem' _ _ _) |- _ => rename H into star end));
+      ((destruct (tsimulation_star props H0 star s3 match_s3) as [s3' [star_sem'' ?]]);
+       assert (init: Smallstep.initial_state sem'' s3) by done).
     - apply (does_FTbc (init) star_sem'').
     - apply (does_FGoes_wrong (init) star_sem'').
       + admit.
@@ -333,19 +531,21 @@ Section Recomposition.
     setoid_rewrite (does_prefix_equiv det_sem').
     setoid_rewrite (does_prefix_equiv det_sem'').
     intros m dp_sem dp_sem' undef_m_ip.
+    pose proof tsim_properties_match_states as props.
     inversion dp_sem; inversion dp_sem';
       try (match goal with | H : (forall s : Smallstep.state _, ~ Smallstep.initial_state _ s) |- _ =>
                                exfalso; eapply H; simpl; unfold initial_state2; unfold initial_state1; eauto end).
-    destruct simulation. remember (initial_state (code prog'') (prog_buffers prog'') (prog_interface prog'')) as s3.
-    assert (match_s3: match_states s s0 s3).
-    { destruct props as [a]. destruct (a _ _ H0 H5) as [s3' [init match_init]]. simpl in init. unfold initial_state3 in init.
+    remember (initial_state (code prog'') (prog_buffers prog'') (prog_interface prog'')) as s3.
+    assert (match_s3: exists M, match_states M s s0 s3).
+    { destruct props as [a]. destruct (a _ _ H0 H5) as [s3' [init match_init]].
+      simpl in init. unfold initial_state3 in init.
       rewrite <- init in Heqs3. subst. done. }
     destruct (tsimulation_star props H1 H6 s3 match_s3) as [s3' [star_sem'' ?]].
     econstructor.
     - simpl; unfold initial_state3; eauto.
-    - eauto. (* we might need to do a few more silent steps in s3'. *)
-    - simpl. intros t' s'' step. admit. (* we should use one of the "diagram properties" here. *)
-    - admit. (* we should use properties of match_states and final_states here. *)
+    - eauto.
+    - admit.
+    - admit.
   Admitted.
 
 End Recomposition.
